Refinery/Term/Extrinsic/Wk.lean
@@ -58,9 +58,204 @@ def Deriv.wk {Γ Δ : Ctx? α} (ρ : Γ.Wk Δ) {A : Ty α} {a : Term φ (Ty α)}
   (D : Δ ⊢ a : A) : (Γ ⊢ a.ren ρ : A)
   := (D.wkD ρ).cast_term (D.wkTerm_eq ρ)
 
+@[simp]
+theorem Deriv.wk_bv {Γ Δ : Ctx? α} (ρ : Γ.Wk Δ) {A : Ty α} {n : ℕ} (x : Δ.At ⟨A, 1⟩ n)
+  : (Deriv.bv x).wk ρ = (Deriv.bv (x.wkIn ρ)) := rfl
+
+@[simp]
+theorem Deriv.wk_op {Γ Δ : Ctx? α} (ρ : Γ.Wk Δ) {A B : Ty α} {a : Term φ (Ty α)}
+  (hf : S.FnTy f A B) (da : Δ ⊢ a : A) : (da.op hf).wk ρ = (da.wk ρ).op hf
+  := by simp [wk, wkD]
+
+@[simp]
+theorem Deriv.wk_let₁ {Γ Δ : Ctx? α} (ρ : Γ.Wk Δ) {A B : Ty α} {a b : Term φ (Ty α)}
+  (hΓ : Δ.SSplit Δl Δr) (da : Δr ⊢ a : A) (db : Δl.cons ⟨A, ⊤⟩ ⊢ b : B)
+  : (da.let₁ hΓ db).wk ρ
+  = ((da.wk (hΓ.rightWk ρ)).cast_term (by simp)).let₁ (hΓ.wk ρ)
+      ((db.wk ((hΓ.leftWk ρ).scons _)).cast_term (by simp))
+  := by simp [wk, wkD]
+
+@[simp]
+theorem Deriv.wk_unit {Γ Δ : Ctx? α} (ρ : Γ.Wk Δ) (hv : Δ.del)
+  : (Deriv.unit hv).wk ρ = Deriv.unit (hv.wk ρ) := rfl
+
+@[simp]
+theorem Deriv.wk_pair {Γ Δ : Ctx? α} (ρ : Γ.Wk Δ) {A B : Ty α} {a b : Term φ (Ty α)}
+  (hΓ : Δ.SSplit Δl Δr) (da : Δl ⊢ a : A) (db : Δr ⊢ b : B)
+  : (da.pair hΓ db).wk ρ
+  = ((da.wk (hΓ.leftWk ρ)).cast_term (by simp)).pair (hΓ.wk ρ)
+      ((db.wk (hΓ.rightWk ρ)).cast_term (by simp))
+  := by simp [wk, wkD]
+
+@[simp]
+theorem Deriv.wk_let₂ {Γ Δ : Ctx? α} (ρ : Γ.Wk Δ) {A B C : Ty α} {a b : Term φ (Ty α)}
+  (hΓ : Δ.SSplit Δl Δr) (da : Δr ⊢ a : A.tensor B) (db : (Δl.cons ⟨A, ⊤⟩).cons ⟨B, ⊤⟩ ⊢ b : C)
+  : (da.let₂ hΓ db).wk ρ
+  = ((da.wk (hΓ.rightWk ρ)).cast_term (by simp)).let₂ (hΓ.wk ρ)
+      ((db.wk (((hΓ.leftWk ρ).scons _).scons _)).cast_term (by simp))
+  := by simp [wk, wkD]
+
+@[simp]
+theorem Deriv.wk_inl {Γ Δ : Ctx? α} (ρ : Γ.Wk Δ) {A B : Ty α} {a : Term φ (Ty α)}
+  (da : Δ ⊢ a : A)
+  : (da.inl (B := B)).wk ρ = (da.wk ρ).inl
+  := by simp [wk, wkD]
+
+@[simp]
+theorem Deriv.wk_inr {Γ Δ : Ctx? α} (ρ : Γ.Wk Δ) {A B : Ty α} {b : Term φ (Ty α)}
+  (db : Δ ⊢ b : B)
+  : (db.inr (A := A)).wk ρ = (db.wk ρ).inr
+  := by simp [wk, wkD]
+
+@[simp]
+theorem Deriv.wk_abort {Γ Δ : Ctx? α} (ρ : Γ.Wk Δ) {A : Ty α} {a : Term φ (Ty α)}
+  (da : Δ ⊢ a : Ty.empty)
+  : (da.abort (A := A)).wk ρ = (da.wk ρ).abort
+  := by simp [wk, wkD]
+
+@[simp]
+theorem Deriv.wk_case {Γ Δ : Ctx? α} (ρ : Γ.Wk Δ) {A B C : Ty α} {a b c : Term φ (Ty α)}
+  (hΓ : Δ.SSplit Δl Δr) (da : Δr ⊢ a : A.coprod B) (db : (Δl.cons ⟨A, ⊤⟩) ⊢ b : C)
+  (dc : (Δl.cons ⟨B, ⊤⟩) ⊢ c : C)
+  : (da.case hΓ db dc).wk ρ
+  = ((da.wk (hΓ.rightWk ρ)).cast_term (by simp)).case (hΓ.wk ρ)
+      ((db.wk ((hΓ.leftWk ρ).scons _)).cast_term (by simp))
+      ((dc.wk ((hΓ.leftWk ρ).scons _)).cast_term (by simp))
+  := by simp [wk, wkD]
+
+@[simp]
+theorem Deriv.wk_iter {Γ Δ : Ctx? α} (ρ : Γ.Wk Δ) {A B : Ty α} {a b : Term φ (Ty α)}
+  (hΓ : Δ.SSplit Δl Δr) (hc : Δl.copy) (hd : Δl.del)
+  (da : Δr ⊢ a : A) (db : Δl.cons ⟨A, ⊤⟩ ⊢ b : B.coprod A)
+  : (da.iter hΓ hc hd db).wk ρ
+  = ((da.wk (hΓ.rightWk ρ)).cast_term (by simp)).iter (hΓ.wk ρ) (hΓ.wkLeft_copy ρ)
+      (hΓ.wkLeft_del ρ) ((db.wk ((hΓ.leftWk ρ).scons _)).cast_term (by simp))
+  := by simp [wk, wkD]
+
+theorem Deriv.wk_eq {Γ Δ : Ctx? α} (ρ ρ' : Γ.Wk Δ) (h : ρ = ρ') {A : Ty α} {a : Term φ (Ty α)}
+  (D : Δ ⊢ a : A) : (D.wk ρ).cast_term (by rw [h]) = D.wk ρ'
+  := by cases h; rfl
+
+theorem Deriv.wk_eq_cast_term
+  {Γ Δ : Ctx? α} (ρ ρ' : Γ.Wk Δ) (h : ρ = ρ') {A : Ty α} {a : Term φ (Ty α)}
+  (ha : a.ren ρ = a') (ha' : a.ren ρ' = a')
+  (D : Δ ⊢ a : A) : (D.wk ρ).cast_term ha = (D.wk ρ').cast_term ha'
+  := by cases h; rfl
+
 def Deriv.pwk {Γ Δ : Ctx? α} (ρ : Γ.PWk Δ) {A : Ty α} {a : Term φ (Ty α)}
   (D : Δ ⊢ a : A) : (Γ ⊢ a : A)
   := (D.wk ρ.toWk).cast_term (by simp [Ctx?.Wk.ix_pwk])
+
+@[simp]
+theorem Deriv.pwk_bv {Γ Δ : Ctx? α} (ρ : Γ.PWk Δ) {A : Ty α} {n : ℕ} (x : Δ.At ⟨A, 1⟩ n)
+  : (Deriv.bv x).pwk ρ = Deriv.bv (x.pwk ρ) := by simp [pwk, Ctx?.At.wkIn_toWk]
+
+@[simp]
+theorem Deriv.pwk_op {Γ Δ : Ctx? α} (ρ : Γ.PWk Δ) {A B : Ty α} {a : Term φ (Ty α)}
+  (hf : S.FnTy f A B) (da : Δ ⊢ a : A) : (da.op hf).pwk ρ = (da.pwk ρ).op hf
+  := by simp [pwk]
+
+@[simp]
+theorem Deriv.pwk_let₁ {Γ Δ : Ctx? α} (ρ : Γ.PWk Δ) {A B : Ty α} {a b : Term φ (Ty α)}
+  (hΓ : Δ.SSplit Δl Δr) (da : Δr ⊢ a : A) (db : Δl.cons ⟨A, ⊤⟩ ⊢ b : B)
+  : (da.let₁ hΓ db).pwk ρ
+  = (da.pwk (hΓ.rightPWk ρ)).let₁ (hΓ.wk ρ.toWk) (db.pwk ((hΓ.leftPWk ρ).scons _))
+  := by
+  simp only [pwk, wk_let₁, cast_term_let₁, cast_term_cast_term]
+  congr 1 <;> apply wk_eq_cast_term <;> simp [Ctx?.SSplit.leftPWk, Ctx?.SSplit.rightPWk]
+
+@[simp]
+theorem Deriv.pwk_let₂ {Γ Δ : Ctx? α} (ρ : Γ.PWk Δ) {A B C : Ty α} {a b : Term φ (Ty α)}
+  (hΓ : Δ.SSplit Δl Δr) (da : Δr ⊢ a : A.tensor B) (db : (Δl.cons ⟨A, ⊤⟩).cons ⟨B, ⊤⟩ ⊢ b : C)
+  : (da.let₂ hΓ db).pwk ρ
+  = (da.pwk (hΓ.rightPWk ρ)).let₂ (hΓ.wk ρ.toWk) (db.pwk (((hΓ.leftPWk ρ).scons _).scons _))
+  := by
+  simp only [pwk, wk_let₂, cast_term_let₂, cast_term_cast_term]
+  congr 1 <;> apply wk_eq_cast_term <;> simp [Ctx?.SSplit.leftPWk, Ctx?.SSplit.rightPWk]
+
+@[simp]
+theorem Deriv.pwk_unit {Γ Δ : Ctx? α} (ρ : Γ.PWk Δ) (hv : Δ.del)
+  : (Deriv.unit hv).pwk ρ = Deriv.unit (hv.wk ρ) := rfl
+
+@[simp]
+theorem Deriv.pwk_pair {Γ Δ : Ctx? α} (ρ : Γ.PWk Δ) {A B : Ty α} {a b : Term φ (Ty α)}
+  (hΓ : Δ.SSplit Δl Δr) (da : Δl ⊢ a : A) (db : Δr ⊢ b : B)
+  : (da.pair hΓ db).pwk ρ
+  = (da.pwk (hΓ.leftPWk ρ)).pair (hΓ.wk ρ.toWk) (db.pwk (hΓ.rightPWk ρ))
+  := by
+  simp only [pwk, wk_pair, cast_term_pair, cast_term_cast_term]
+  congr 1 <;> apply wk_eq_cast_term <;> simp [Ctx?.SSplit.leftPWk, Ctx?.SSplit.rightPWk]
+
+@[simp]
+theorem Deriv.pwk_inl {Γ Δ : Ctx? α} (ρ : Γ.PWk Δ) {A B : Ty α} {a : Term φ (Ty α)}
+  (da : Δ ⊢ a : A)
+  : (da.inl (B := B)).pwk ρ = (da.pwk ρ).inl
+  := by simp [pwk]
+
+@[simp]
+theorem Deriv.pwk_inr {Γ Δ : Ctx? α} (ρ : Γ.PWk Δ) {A B : Ty α} {b : Term φ (Ty α)}
+  (db : Δ ⊢ b : B)
+  : (db.inr (A := A)).pwk ρ = (db.pwk ρ).inr
+  := by simp [pwk]
+
+@[simp]
+theorem Deriv.pwk_abort {Γ Δ : Ctx? α} (ρ : Γ.PWk Δ) {A : Ty α} {a : Term φ (Ty α)}
+  (da : Δ ⊢ a : Ty.empty)
+  : (da.abort (A := A)).pwk ρ = (da.pwk ρ).abort
+  := by simp [pwk]
+
+@[simp]
+theorem Deriv.pwk_case {Γ Δ : Ctx? α} (ρ : Γ.PWk Δ) {A B C : Ty α} {a b c : Term φ (Ty α)}
+  (hΓ : Δ.SSplit Δl Δr) (da : Δr ⊢ a : A.coprod B) (db : (Δl.cons ⟨A, ⊤⟩) ⊢ b : C)
+  (dc : (Δl.cons ⟨B, ⊤⟩) ⊢ c : C)
+  : (da.case hΓ db dc).pwk ρ
+  = (da.pwk (hΓ.rightPWk ρ)).case (hΓ.wk ρ.toWk) (db.pwk ((hΓ.leftPWk ρ).scons _))
+      (dc.pwk ((hΓ.leftPWk ρ).scons _))
+  := by
+  simp only [pwk, wk_case, cast_term_case, cast_term_cast_term]
+  congr 1 <;> apply wk_eq_cast_term <;> simp [Ctx?.SSplit.leftPWk, Ctx?.SSplit.rightPWk]
+
+@[simp]
+theorem Deriv.pwk_iter {Γ Δ : Ctx? α} (ρ : Γ.PWk Δ) {A B : Ty α} {a b : Term φ (Ty α)}
+  (hΓ : Δ.SSplit Δl Δr) (hc : Δl.copy) (hd : Δl.del)
+  (da : Δr ⊢ a : A) (db : Δl.cons ⟨A, ⊤⟩ ⊢ b : B.coprod A)
+  : (da.iter hΓ hc hd db).pwk ρ
+  = (da.pwk (hΓ.rightPWk ρ)).iter (hΓ.wk ρ.toWk) (hΓ.wkLeft_copy ρ.toWk) (hΓ.wkLeft_del ρ.toWk)
+      (db.pwk ((hΓ.leftPWk ρ).scons _))
+  := by
+  simp only [pwk, wk_iter, cast_term_iter, cast_term_cast_term]
+  congr 1 <;> apply wk_eq_cast_term <;> simp [Ctx?.SSplit.leftPWk, Ctx?.SSplit.rightPWk]
+
+-- theorem Deriv.wk_heq_ofEq {Γ Δ : Ctx? α} (h : Γ = Δ) {A : Ty α} {a : Term φ (Ty α)}
+--   (D : Δ ⊢ a : A) : HEq (D.wk (.ofEq h)) D
+--   := by induction a generalizing Γ Δ A with
+--   | let₁ _ _ _ Ia Ib =>
+--     cases D
+--     simp? [ren.eq_3, wk_let₁, Ctx?.Wk.ix.eq_2]
+--     congr
+--     simp
+--     simp
+--     sorry
+--   | _ => sorry
+
+
+-- theorem Deriv.wk_ofEq {Γ Δ : Ctx? α} (h : Γ = Δ) {A : Ty α} {a : Term φ (Ty α)}
+--   (D : Δ ⊢ a : A) : D.wk (.ofEq h) = D.cast h.symm rfl (by cases h; simp)
+--   := by induction a generalizing Γ Δ A with
+--   | let₁ _ _ _ Ia Ib =>
+--     cases D
+--     simp only [ren, wk_let₁, Ctx?.Wk.ix.eq_2, cast_let₁, let₁.injEq, Ctx?.SSplit.wkLeft_ofEq,
+--       Ctx?.SSplit.wkRight_ofEq, true_and]
+--     sorry
+--   | _ => sorry
+
+-- def Deriv.pwk_ofEq {Γ Δ : Ctx? α} (h : Γ = Δ) {A : Ty α} {a : Term φ (Ty α)}
+--   (D : Δ ⊢ a : A) : D.pwk (.ofEq h) = D.cast_ctx h.symm
+--   := by induction D <;> simp [*]
+
+-- def Deriv.pwk_refl {Γ Δ : Ctx? α} {A : Ty α} {a : Term φ (Ty α)}
+--   (D : Γ ⊢ a : A) : D.pwk (Ctx?.PWk.refl Γ) = D
+--   := by induction D <;> simp [*]
 
 end Term
 
